Extra control flow total tweak
git-svn-id: orca@252

WP1-Programming-Languages-Semantics/WP11-C-semantics/src/IMP-Lenses/hoare/VCG_total_ML.thy
@@ -8,10 +8,10 @@ text \<open>@{text \<open>infixl\<close>} rather than @{text \<open>infixr\<clos
 no_notation useq (infixr ";;" 51)
 notation useq (infixl ";;" 51)
 
-text \<open>@{thm seq_hoare_r_t} and @{thm assigns_hoare_r_t} are handled separately as they could cause
-conflicts/failed proofs later on.\<close>
-lemmas vcg_rules = skip_hoare_r_t cond_hoare_r_t assigns_hoare_r'_t assert_hoare_r_t
-assume_hoare_r_t while_invr_hoare_r_t while_hoare_r_t while_hoare_r'_t
+text \<open>@{thm seq_hoare_r_t}, @{thm assigns_hoare_r_t}, @{thm while_invr_hoare_r_t}, and
+@{thm cond_hoare_r_t} are handled separately as they could cause conflicts/failed proofs later on.\<close>
+lemmas vcg_rules = skip_hoare_r_t assigns_hoare_r'_t assert_hoare_r_t assume_hoare_r_t
+while_hoare_r_t while_hoare_r'_t
 lemmas unfold_thms = lens_indep_def
 
 text \<open>Examples of breaking down theorems as terms\<close>
@@ -29,14 +29,16 @@ rassume_c |> Thm.concl_of |> HOLogic.dest_Trueprop |> HOLogic.dest_eq |> fst
 (* Need to start with seq splitting, applying the `seq_hoare_r_t[of _ _ true]` step when an
 assumption is the last command in a goal; then we can apply other rules and such. When we encounter
 while loops and if statements we have to try seq splitting again after while/if application as those
-statements can have nested sequences of commands (including more while/if statements).
-Tricky tricky. *)
+statements can have nested sequences of commands (including more while/if statements). *)
 
 (* FIRST' isn't necessary if you only have one tactic to try; it's meant for lists of tactics.
 However, it seems the below setups would need to be revised some other way to use without FIRST'.*)
 ML \<open>
 fun pprint_term ctxt term = Pretty.writeln (Syntax.pretty_term ctxt term)
 fun pprint_cterm ctxt cterm = pprint_term ctxt (Thm.term_of cterm)
+
+fun dest_hoare_rd (Const (@{const_name hoare_rd}, _) $ _ $ P $ _) = P
+  | dest_hoare_rd t = raise TERM ("dest_hoare_rd", [t]);
 
 (* ML-level version of `seq_hoare_r_t[of _ _ true]`; there's also (Drule.)infer_instantiate', but
 that requires a proof context. *)
@@ -47,19 +49,32 @@ val seq_hoare_r_t' =
 is the last command in a goal.
 Subgoal.focus elements: {prems, params, asms, concl, context, schematics} *)
 fun vcg_seq_split ctxt goal = (REPEAT o CHANGED) (Subgoal.FOCUS (fn {concl, ...} =>
-  case concl |> Thm.term_of |> HOLogic.dest_Trueprop of
-    Const (@{const_name hoare_rd}, _) $ _ $
-      (Const (@{const_name seqr}, _) $ _ $
-        (Const (@{const_name rassume_c}, _) $ _)) $
-    _ => resolve_tac ctxt [seq_hoare_r_t'] goal |
-    _ => resolve_tac ctxt @{thms seq_hoare_r_t} goal
-  ) ctxt goal)
+  case concl |> Thm.term_of |> HOLogic.dest_Trueprop |> dest_hoare_rd of
+    Const (@{const_name seqr}, _) $ _ $
+      (Const (@{const_name rassume_c}, _) $ _)
+        => resolve_tac ctxt [seq_hoare_r_t'] goal |
+    _ => resolve_tac ctxt @{thms seq_hoare_r_t} goal)
+  ctxt goal)
 
 (* Handles applying most Hoare rules, with the specific exclusion of seq_hoare_r_t and
-assigns_hoare_r_t; match_tac (equivalent to `intro`) may be a better choice. *)
-(* fun vcg_resolve_tac ctxt = (ALLGOALS o REPEAT_ALL_NEW) (CHANGED o TRY o FIRST'
-                           [resolve_tac ctxt @{thms vcg_rules}]) *)
-fun vcg_resolve_tac ctxt goal = (REPEAT o CHANGED) (resolve_tac ctxt @{thms vcg_rules} goal)
+assigns_hoare_r_t [though one version calls through to it just in case]
+(try match_tac (equivalent to `intro`) rather than resolve_tac (equivalent to `rule`)?)
+Using Subgoal.FOCUS
+messes up the behavior when goals should merge due to certain rules like the skip rule, etc. that
+work fine when FOCUS is not used. *)
+fun vcg_rule_tac ctxt goal = (REPEAT o CHANGED) (resolve_tac ctxt @{thms vcg_rules} goal)
+
+fun vcg_rule_wc_tac ctxt goal = (REPEAT o CHANGED) (Subgoal.FOCUS (fn {concl, ...} =>
+  case concl |> Thm.term_of |> HOLogic.dest_Trueprop |> dest_hoare_rd of
+    Const (@{const_name While_inv}, _) $ _ $ _ $ _
+      => (resolve_tac ctxt @{thms while_invr_hoare_r_t} goal THEN vcg_seq_split ctxt goal) |
+    Const (@{const_name trop}, _) $
+      Const (@{const_name If}, _) $ _ $ _ $ _
+        => (resolve_tac ctxt @{thms cond_hoare_r_t} goal THEN (* need to handle both cond goals *)
+            vcg_seq_split ctxt goal THEN
+            vcg_seq_split ctxt (goal + 1)) |
+    _ => no_tac)
+  ctxt goal)
 
 (* Equivalent to `apply (insert assms)`;
 not needed for rule application, only some {rel,pred}_* usage *)
@@ -69,7 +84,7 @@ fun vcg_insert_assms_tac ctxt = (ALLGOALS o FIRST')
 (* Must come before certain usages of {rel,pred}_*  *)
 fun vcg_unfold_tac ctxt = unfold_tac ctxt @{thms unfold_thms}
 
-val vcg_tac =(*  vcg_resolve_tac THEN' *)
+val vcg_tac =(*  vcg_rule_tac THEN' *)
               vcg_insert_assms_tac THEN'
               (* apply rules, but with specific handling for the assumes/etc. cases;
               may also want to stick with partial rule application so we can
@@ -115,12 +130,14 @@ lemma increment_tactic:
   \<lbrace>&x =\<^sub>u 5\<rbrace>\<^sub>D"
   apply (tactic \<open>vcg_seq_split @{context} 1\<close>)
   apply rel_auto
-  apply (tactic \<open>vcg_resolve_tac @{context} 1\<close>)
+  apply (tactic \<open>vcg_rule_tac @{context} 1\<close>)
+  apply rel_auto
+  apply (tactic \<open>vcg_rule_wc_tac @{context} 1\<close>)
   apply rel_auto
 oops
-
+term "II"
 ML \<open>
-@{term "\<lbrace>p\<rbrace>C;;a\<^sup>\<top>\<^sup>C\<lbrace>q\<rbrace>\<^sub>D"};
+@{term "while b invr i do c od"};
 pprint_cterm @{context} @{cterm "\<lbrace>p\<rbrace>C;;c\<^sup>\<top>\<^sup>C\<lbrace>q\<rbrace>\<^sub>D"}
 \<close>
 
